\appendix
\chapter{Appendix}
\section{The Yukawa interaction term for right-handed neutrinos}
\chapter{}
\section{Calculations}
\begin{equation*}
(\frac{d}{dt}+3H)n_N=-\Gamma_N(n_N-n_N^{eq})+\underbrace{\Gamma_{N,B-L}n_{B-L}}_\text{negligible}
\end{equation*}
phase space integral
\begin{align*}
\int (\frac{d}{dt}+3H)f_Nd^3p=-\int\Gamma_N(f_N-f_N^{eq})d^3p\\
\int (\frac{d}{dt}+3H)f_Np^2dp=-\int\Gamma_N(f_N-f_N^{eq})^2dp
\end{align*}
Using
\begin{equation*}
\int p^3\frac{\partial f_N}{\partial p}dp=\left[p^3f_N\right]_0^\infty-3\int p^2f_Ndp=-3\int p^2f_Ndp
\end{equation*}
\begin{equation*}
3H\int f_Np^2dp=-H\int p^3\frac{\partial f_N}{\partial p}dp
\end{equation*}
it follows
\begin{align*}
\int (\partial_t-Hp\partial_p)f_Np^2dp&=-\int\Gamma_N(f_N-f_N^{eq})p^2dp\\
\Rightarrow (\partial_t-Hp\partial_p)f_N&=\Gamma_N(f_N^{eq}-f_N)
\end{align*}
\newpage
\begin{align*}
	n_l-n_{\bar{l}}&=\int\frac{d^3p}{(2\pi)^3}f_l-f_{\bar{l}}=\\
	&=\frac{1}{(2\pi)^3}\int (f_l-f_{\bar{l}})p^2\:dp\:dcos\theta \:d\phi=\\
	&=\frac{1}{2\pi^2}\int\left(f_l(\mu_l=0)+\frac{e^{E/T}}{(e^{E/T}+1)^2T}\mu_l-f_{\bar{l}}(\mu_{\bar{l}}=0)-\frac{e^{E/T}}{(e^{E/T}+1)^2T}\mu_{\bar{l}}\right)p^2\:dp=\\
	&=\frac{1}{2\pi^2}\int\frac{2e^{E/T}}{(e^{E/T}+1)^2T}\mu_l\:p^2\:dp=\\
	&=\frac{\mu_l}{\pi^2T}\underbrace{\int_{0}^{\infty}\frac{2e^{E/T}}{(e^{E/T}+1)^2}\:E^2\:dE}_{=\frac{\pi^2T^3}{6}}=\\
	&=\frac{\mu_lT^2}{6}
\end{align*}
Analogous calculation for the Higgs yields:
\begin{align*}
	n_\phi-n_{\bar{\phi}}=\frac{\mu_lT^2}{3}
\end{align*}
Solving
\begin{align*}
	n_l-n_{\bar{l}}=-c_ln_{B-L}\\
	n_\phi-n_{\bar{\phi}}=-c_\phi n_{B-L}
\end{align*}
for the chemical potentials yields
\begin{align*}
	\mu_l=-\frac{6c_l}{T^2}n_{B-L}\neq\frac{3c_l}{T^2}n_{B-L}\\
	\mu_\phi=-\frac{3c_\phi}{T^2}n_{B-L}\neq\frac{3c_l}{2T^2}n_{B-L}
\end{align*}
\newpage
\begin{equation*}
	\Gamma_{B-L}n_{B-L}=\int\prod_{a=N,l,\phi}\frac{d^3p_a}{2E_a(2\pi)^3}(2\pi^4)\delta(p_l+p_\phi-p_N)(	f_lf_\phi-f_{\bar{l}}f_{\bar{\phi}})\sum|M_0|^2
\end{equation*}
\newline
\begin{equation*}
	f_l^{eq}f_\phi^{eq}=e^{-\frac{E_l-\mu_l}{T}}e^{-\frac{E_\phi-\mu_\phi}{T}}\overset{E_l+E_\phi=E_N}{=}e^{-\frac{E_N-\mu_l-\mu_\phi}{T}}=e^{-\frac{E_N}{T}}e^{\frac{\mu_l+\mu_\phi}{T}}
\end{equation*}
\begin{equation*}
	f_lf_\phi\simeq e^{-\frac{E_N}{T}}\left(1+\frac{\mu_l+\mu_\phi}{T}\right)
\end{equation*}
\begin{equation*}
	f_lf_\phi-f_{\bar{l}}f_{\bar{\phi}}\simeq e^{-\frac{E_N}{T}}\left(1+\frac{\mu_l+\mu_\phi}{T}-1-\frac{\mu_{\bar{l}}+\mu_{\bar{\phi}}}{T}\right)\overset{\mu_X=-\mu_{\bar{X}}}{=}2e^{-\frac{E_N}{T}}\frac{\mu_l+\mu_\phi}{T}
\end{equation*}

\newpage